Source/DafnyCore/Backends/Python/PythonCodeGenerator.cs
@@ -1,7 +1,6 @@
 using System;
 using System.Collections.Generic;
 using System.Diagnostics.Contracts;
-using System.IO;
 using System.Linq;
 using System.Numerics;
 using DafnyCore.Backends.Python;
